UnfoldReify.fst
@@ -1,0 +1,108 @@
+module UnfoldReify
+
+open FStar.Exn
+open FStar.Tactics
+
+type maybe (a:Type) = either a exn 
+
+type m4 (a:Type) = 
+| Return : a -> m4 a
+
+let m4_return (a:Type) (x: a) : m4 a = Return x
+
+let m4_bind (a:Type) (b:Type) (l:m4 a) (k:a -> m4 b) : m4 b =
+  match l with
+  | Return x -> k x
+
+let m4_post a = maybe a -> Type0
+let m4_wpty a = m4_post a -> Type0
+
+let m4_return_wp (a:Type) (x:a) : m4_wpty a = fun p -> p (Inl x) 
+
+let compute_post (a b:Type) (km4_wpty : a -> m4_wpty b) (p:m4_post b) : m4_post a =
+      (fun result -> 
+        match result with
+        | Inl v -> km4_wpty v (fun r' -> p r')
+        | Inr err -> p (Inr err))
+
+let m4_bind_wp (a b:Type) (w : m4_wpty a) (kw : a -> m4_wpty b) : m4_wpty b =
+  fun p -> w (compute_post a b kw p)
+
+let m4_interpretation #a (m : m4 a) (p : m4_post a) : Type0 = True
+
+let irepr (a:Type) (wp:m4_wpty a) =
+  post:m4_post a ->
+    Pure (m4 a)
+      (requires (wp post))
+      (ensures (fun (t:m4 a) -> m4_interpretation t post))
+
+let ireturn (a : Type) (x : a) : irepr a (m4_return_wp a x) = fun _ -> m4_return a x
+
+val w_ord (#a : Type) : m4_wpty a -> m4_wpty a -> Type0
+let w_ord wp1 wp2 = forall p. wp1 p ==> wp2 p
+
+let ibind (a b : Type) (wp_v : m4_wpty a) (wp_f: a -> m4_wpty b) (v : irepr a wp_v)
+  (f : (x:a -> irepr b (wp_f x))) : irepr b (m4_bind_wp _ _ wp_v wp_f) =
+  fun p -> 
+    let t = (m4_bind a b
+        (v (compute_post a b wp_f p))
+        (fun x ->
+          assume (wp_f x p);
+           f x p)) in
+    assume (m4_interpretation t p);
+    t
+
+let isubcomp (a:Type) (wp1 wp2: m4_wpty a) (f : irepr a wp1) :
+  Pure (irepr a wp2) (requires w_ord wp2 wp1) (ensures fun _ -> True) = f
+
+let wp_if_then_else (#a:Type) (wp1 wp2:m4_wpty a) (b:bool) : m4_wpty a =
+  fun p -> (b ==> wp1 p) /\ ((~b) ==> wp2 p)
+
+let i_if_then_else (a : Type) (wp1 wp2 : m4_wpty a) (f : irepr a wp1) (g : irepr a wp2) (b : bool) : Type =
+  irepr a (wp_if_then_else wp1 wp2 b)
+
+total
+reifiable
+reflectable
+layered_effect {
+  M4wp : a:Type -> wp : m4_wpty a -> Effect
+  with
+       repr       = irepr
+     ; return     = ireturn
+     ; bind       = ibind
+
+     ; subcomp      = isubcomp
+     ; if_then_else = i_if_then_else
+}
+  
+let elim_pure #a #wp ($f : unit -> PURE a wp) p
+ : Pure a (requires (wp p)) (ensures (fun r -> p r))
+ = FStar.Monotonic.Pure.wp_monotonic_pure (); f ()
+
+let lift_pure_m4wp (a:Type) (wp:pure_wp a) (f:(eqtype_as_type unit -> PURE a wp)) :
+  Pure (irepr a (fun p -> wp (fun r -> p (Inl r)))) (requires True)
+                    (ensures (fun _ -> True))
+  = fun p -> let r = elim_pure f (fun r -> p (Inl r)) in m4_return _ r
+
+sub_effect PURE ~> M4wp = lift_pure_m4wp
+
+
+let to_option #t1 (x:t1) : option t1 = Some x
+
+let test (x:int) = lift_pure_m4wp (option int) (fun p -> p (to_option x)) (fun _ -> to_option x)
+
+let lemma
+  #t1 #t2
+  (wp : m4_wpty t2)
+  (f:irepr t2 wp)
+  (p:m4_post (option t2)) : 
+  Lemma (requires (forall p. wp p))
+    (ensures (true == true)) =
+    calc (==) {
+      reify (to_option (M4wp?.reflect f) <: option t2);
+      == { admit () }
+      ibind t2 (option t2) wp (fun x -> m4_return_wp (option t2) (to_option x))
+        (reify (M4wp?.reflect f))
+        (fun x -> lift_pure_m4wp (option t2) (fun p -> p (to_option x)) (fun _ -> to_option x))
+        ;
+    }
